nn.v moved to Type

yalla/nn.v
@@ -14,9 +14,11 @@ Require Import Omega.
 Require Import Injective.
 Require Import Bool_more.
 Require Import List_more.
-Require Import Permutation_more.
-Require Import Permutation_solve.
-Require Import genperm.
+Require Import List_Type.
+Require Import List_Type_more.
+Require Import Permutation_Type_more.
+Require Import Permutation_Type_solve.
+Require Import genperm_Type.
 
 Require Import subs.
 Require Import isubs.
@@ -35,8 +37,8 @@ Definition i2ac := yalla_ax.i2ac.
 Definition i2ac_inj := yalla_ax.i2ac_inj.
 Definition ateq_a2i := yalla_ax.ateq_a2i.
 
-Definition ipfrag_ill := mk_ipfrag true (fun _ _ => False) true.
-(*                                 cut   axioms            perm  *)
+Definition ipfrag_ill := mk_ipfrag true NoIAxioms true.
+(*                                 cut  axioms    perm  *)
 Definition ill_ll := ill ipfrag_ill.
 
 Definition unill := ill2ll i2a.
@@ -46,7 +48,7 @@ Definition unill := ill2ll i2a.
 Section RTranslation.
 
 Context {P : pfrag}.
-Hypothesis P_axfree : forall l, ~ pgax P l.
+Hypothesis P_axfree : forall a : projT1 (pgax P), False.
 Hypothesis P_perm : pperm P = true.
 
 (** We fix the parameter [R] of the translation. *)
@@ -54,21 +56,21 @@ Hypothesis P_perm : pperm P = true.
 Variable R : iformula.
 Definition negR A := ilmap A R.
 
-Lemma negR_irr : forall A l s,
-  ill_ll (A :: l) R s -> ill_ll l (negR A) (S s).
+Lemma negR_irr : forall A l,
+  ill_ll (A :: l) R -> ill_ll l (negR A).
 Proof.
-intros A l s pi.
+intros A l pi.
 apply lmap_irr.
 assumption.
 Qed.
 
-Lemma negR_ilr : forall sR, ill_ll (R :: nil) R sR ->
-  forall A l s, ill_ll l A s -> ill_ll (negR A :: l) R (S (S (s + sR))).
+Lemma negR_ilr : ill_ll (R :: nil) R ->
+  forall A l, ill_ll l A -> ill_ll (negR A :: l) R.
 Proof.
-intros sR HR A l s pi.
+intros HR A l pi.
 rewrite <- (app_nil_r _).
 rewrite <- app_comm_cons.
-eapply ex_ir ; [ | symmetry ; apply Permutation_middle ].
+eapply ex_ir ; [ | symmetry ; apply Permutation_Type_middle ].
 rewrite <- (app_nil_l _).
 apply lmap_ilr ; assumption.
 Qed.
@@ -98,7 +100,7 @@ induction l...
 simpl ; rewrite IHl...
 Qed.
 
-Lemma trans_nz : ~ zeropos R -> nonzerospos R ->
+Lemma trans_nz : (zeropos R -> False) -> nonzerospos R ->
   forall A, nonzerospos (trans A).
 Proof with myeasy.
 intros Hnz Hnzsp.
@@ -106,15 +108,11 @@ induction A ; simpl ; try now constructor ;
   try (constructor ; try assumption ; now constructor).
 Qed.
 
-Lemma neg_tens_propag : forall A1 A2 B1 B2 s1 s2,
-  ill_ll (A1 :: negR A2 :: nil) R s1 -> ill_ll (B1 :: negR B2 :: nil) R s2 -> 
-    exists s, ill_ll (itens A1 B1 :: negR (itens A2 B2) :: nil) R s.
+Lemma neg_tens_propag : forall A1 A2 B1 B2,
+  ill_ll (A1 :: negR A2 :: nil) R -> ill_ll (B1 :: negR B2 :: nil) R ->
+    ill_ll (itens A1 B1 :: negR (itens A2 B2) :: nil) R.
 Proof with myeeasy.
-intros A1 A2 B1 B2 s1 s2 pi1 pi2.
-destruct (@ax_exp_ill ipfrag_ill R) as [sR axR].
-destruct (@ax_exp_ill ipfrag_ill A2) as [sA2 axA2].
-destruct (@ax_exp_ill ipfrag_ill B2) as [sB2 axB2].
-eexists.
+intros A1 A2 B1 B2 pi1 pi2.
 cons2app.
 rewrite <- (app_nil_l _).
 eapply (cut_ir _ (itens (negR (negR A2)) (negR (negR B2))))...
@@ -122,8 +120,8 @@ eapply (cut_ir _ (itens (negR (negR A2)) (negR (negR B2))))...
   apply tens_ilr.
   list_simpl ; cons2app.
   apply tens_irr ; apply lmap_irr.
-  + eapply ex_ir ; [ apply pi1 | apply perm_swap ]...
-  + eapply ex_ir ; [ apply pi2 | apply perm_swap ]...
+  + eapply ex_ir ; [ apply pi1 | apply Permutation_Type_swap ]...
+  + eapply ex_ir ; [ apply pi2 | apply Permutation_Type_swap ]...
 - list_simpl.
   rewrite <- (app_nil_l _).
   apply tens_ilr.
@@ -131,31 +129,30 @@ eapply (cut_ir _ (itens (negR (negR A2)) (negR (negR B2))))...
   rewrite <- (app_nil_l (negR (itens _ _) :: _)).
   rewrite 2 app_comm_cons.
   rewrite <- (app_nil_l _).
-  apply negR_ilr...
-  apply negR_irr.
-  eapply ex_ir ; [ | apply perm_swap ].
-  apply negR_ilr...
-  apply negR_irr.
-  cons2app.
-  rewrite app_assoc.
-  eapply ex_ir ; [ | apply Permutation_middle ].
-  list_simpl.
-  apply negR_ilr...
-  eapply ex_ir ; [ | apply perm_swap ].
-  cons2app.
-  apply tens_irr...
+  apply negR_ilr.
+  + apply ax_exp_ill.
+  + apply negR_irr.
+    eapply ex_ir ; [ | apply Permutation_Type_swap ].
+    apply negR_ilr...
+    * apply ax_exp_ill.
+    * apply negR_irr.
+      cons2app.
+      rewrite app_assoc.
+      eapply ex_ir ; [ | apply Permutation_Type_middle ].
+      list_simpl.
+      apply negR_ilr...
+      -- apply ax_exp_ill.
+      -- eapply ex_ir ; [ | apply Permutation_Type_swap ].
+         cons2app.
+         apply tens_irr ; apply ax_exp_ill.
 Unshelve. reflexivity.
 Qed.
 
-Lemma neg_plus_propag : forall A1 A2 B1 B2 s1 s2,
-  ill_ll (A1 :: negR A2 :: nil) R s1 -> ill_ll (B1 :: negR B2 :: nil) R s2 -> 
-    exists s, ill_ll (iplus A1 B1 :: negR (iplus A2 B2) :: nil) R s.
+Lemma neg_plus_propag : forall A1 A2 B1 B2,
+  ill_ll (A1 :: negR A2 :: nil) R -> ill_ll (B1 :: negR B2 :: nil) R ->
+    ill_ll (iplus A1 B1 :: negR (iplus A2 B2) :: nil) R.
 Proof with myeeasy.
-intros A1 A2 B1 B2 s1 s2 pi1 pi2.
-destruct (@ax_exp_ill ipfrag_ill R) as [sR axR].
-destruct (@ax_exp_ill ipfrag_ill A2) as [sA2 axA2].
-destruct (@ax_exp_ill ipfrag_ill B2) as [sB2 axB2].
-eexists.
+intros A1 A2 B1 B2 pi1 pi2.
 cons2app.
 rewrite <- (app_nil_l _).
 eapply (cut_ir _ (iplus (negR (negR A2)) (negR (negR B2))))...
@@ -164,73 +161,46 @@ eapply (cut_ir _ (iplus (negR (negR A2)) (negR (negR B2))))...
   + list_simpl.
     apply plus_irr1.
     apply negR_irr.
-    eapply ex_ir ; [ | apply perm_swap ]...
+    eapply ex_ir ; [ | apply Permutation_Type_swap ]...
   + list_simpl.
     apply plus_irr2.
     apply negR_irr.
-    eapply ex_ir ; [ | apply perm_swap ]...
+    eapply ex_ir ; [ | apply Permutation_Type_swap ]...
 - list_simpl.
   rewrite <- (app_nil_l _).
   apply plus_ilr.
   + list_simpl.
-    apply negR_ilr...
-    apply negR_irr.
-    eapply ex_ir ; [ | apply perm_swap ].
-    apply negR_ilr...
-    apply plus_irr1...
+    apply negR_ilr.
+    * apply ax_exp_ill.
+    * apply negR_irr.
+      eapply ex_ir ; [ | apply Permutation_Type_swap ].
+      apply negR_ilr.
+      -- apply ax_exp_ill.
+      -- apply plus_irr1.
+         apply ax_exp_ill.
   + list_simpl.
-    apply negR_ilr...
-    apply negR_irr.
-    eapply ex_ir ; [ | apply perm_swap ].
-    apply negR_ilr...
-    apply plus_irr2...
+    apply negR_ilr.
+    * apply ax_exp_ill.
+    * apply negR_irr.
+      eapply ex_ir ; [ | apply Permutation_Type_swap ].
+      apply negR_ilr.
+      -- apply ax_exp_ill.
+      -- apply plus_irr2.
+         apply ax_exp_ill.
 Unshelve. reflexivity.
 Qed.
 
-Lemma trans_dual : forall A, exists s,
-  ill_ll (negR (trans A) :: negR (trans (dual A)) :: nil) R s.
-Proof with myeeasy.
-destruct (@ax_exp_ill ipfrag_ill R) as [sR axR].
-induction A ;
-  try destruct IHA as [s0 IHA] ;
-  try destruct IHA1 as [s1 IHA1] ;
-  try destruct IHA2 as [s2 IHA2] ;
-  simpl.
-- eexists.
+Lemma trans_dual : forall A,
+  ill_ll (negR (trans A) :: negR (trans (dual A)) :: nil) R.
+Proof with myeeasy ; try now (apply ax_exp_ill).
+induction A ; simpl.
+- apply negR_ilr...
+- eapply ex_ir ; [ | apply Permutation_Type_swap ].
   apply negR_ilr...
-  apply negR_irr.
-  eapply ex_ir ; [ | apply perm_swap ].
+- apply negR_ilr...
+- eapply ex_ir ; [ | apply Permutation_Type_swap ].
   apply negR_ilr...
-  apply ax_ir.
-- eexists.
-  eapply ex_ir ; [ | apply perm_swap ].
-  apply negR_ilr...
-  apply negR_irr.
-  eapply ex_ir ; [ | apply perm_swap ].
-  apply negR_ilr...
-  apply ax_ir.
-- eexists.
-  apply negR_ilr...
-  apply negR_irr.
-  eapply ex_ir ; [ | apply perm_swap ].
-  apply negR_ilr...
-  rewrite <- (app_nil_l _).
-  apply one_ilr.
-  apply one_irr.
-- eexists.
-  eapply ex_ir ; [ | apply perm_swap ].
-  apply negR_ilr...
-  apply negR_irr.
-  eapply ex_ir ; [ | apply perm_swap ].
-  apply negR_ilr...
-  rewrite <- (app_nil_l _).
-  apply one_ilr.
-  apply one_irr.
-- destruct (@ax_exp_ill ipfrag_ill (negR (trans A1))) as [sA1 axA1].
-  destruct (@ax_exp_ill ipfrag_ill (negR (trans A2))) as [sA2 axA2].
-  apply (neg_tens_propag _ _ _ _ _ _ IHA2) in IHA1.
-  destruct IHA1 as [s IHA1].
-  eexists.
+- apply (neg_tens_propag _ _ _ _ IHA2) in IHA1.
   apply negR_ilr...
   apply negR_irr.
   cons2app.
@@ -239,17 +209,13 @@ induction A ;
   rewrite <- (app_nil_l _).
   apply tens_ilr.
   list_simpl.
-  eapply ex_ir ; [ | apply perm_swap ].
+  eapply ex_ir ; [ | apply Permutation_Type_swap ].
   cons2app.
   apply tens_irr...
-- destruct (@ax_exp_ill ipfrag_ill (negR (trans (dual A1)))) as [sA1 axA1].
-  destruct (@ax_exp_ill ipfrag_ill (negR (trans (dual A2)))) as [sA2 axA2].
-  eapply ex_ir in IHA1 ; [ | apply perm_swap ].
-  eapply ex_ir in IHA2 ; [ | apply perm_swap ].
-  apply (neg_tens_propag _ _ _ _ _ _ IHA1) in IHA2.
-  destruct IHA2 as [s IHA2].
-  eexists.
-  eapply ex_ir ; [ | apply perm_swap ].
+- eapply ex_ir in IHA1 ; [ | apply Permutation_Type_swap ].
+  eapply ex_ir in IHA2 ; [ | apply Permutation_Type_swap ].
+  apply (neg_tens_propag _ _ _ _ IHA1) in IHA2.
+  eapply ex_ir ; [ | apply Permutation_Type_swap ].
   apply negR_ilr...
   apply negR_irr.
   cons2app.
@@ -258,59 +224,30 @@ induction A ;
   rewrite <- (app_nil_l _).
   apply tens_ilr.
   list_simpl.
-  eapply ex_ir ; [ | apply perm_swap ].
+  eapply ex_ir ; [ | apply Permutation_Type_swap ].
   cons2app.
   apply tens_irr...
-- eexists.
+- apply negR_ilr...
+- eapply ex_ir ; [ | apply Permutation_Type_swap ].
   apply negR_ilr...
-  apply negR_irr.
-  rewrite <- (app_nil_l _).
-  apply zero_ilr.
-- eexists.
-  eapply ex_ir ; [ | apply perm_swap ].
-  apply negR_ilr...
-  apply negR_irr.
-  rewrite <- (app_nil_l _).
-  apply zero_ilr.
-- destruct (@ax_exp_ill ipfrag_ill (negR (trans A1))) as [sA1 axA1].
-  destruct (@ax_exp_ill ipfrag_ill (negR (trans A2))) as [sA2 axA2].
-  apply (neg_plus_propag _ _ _ _ _ _ IHA1) in IHA2.
-  destruct IHA2 as [s IHA2].
-  eexists.
+- apply (neg_plus_propag _ _ _ _ IHA1) in IHA2.
   apply negR_ilr...
   apply negR_irr.
   cons2app.
   rewrite <- (app_nil_l _).
   eapply cut_ir ; [ | | apply IHA2 ]...
-  rewrite <- (app_nil_l _).
-  apply plus_ilr.
-  + list_simpl.
-    apply plus_irr1...
-  + list_simpl.
-    apply plus_irr2...
-- destruct (@ax_exp_ill ipfrag_ill (negR (trans (dual A1)))) as [sA1 axA1].
-  destruct (@ax_exp_ill ipfrag_ill (negR (trans (dual A2)))) as [sA2 axA2].
-  eapply ex_ir in IHA1 ; [ | apply perm_swap ].
-  eapply ex_ir in IHA2 ; [ | apply perm_swap ].
-  apply (neg_plus_propag _ _ _ _ _ _ IHA1) in IHA2.
-  destruct IHA2 as [s IHA2].
-  eexists.
-  eapply ex_ir ; [ | apply perm_swap ].
+- eapply ex_ir in IHA1 ; [ | apply Permutation_Type_swap ].
+  eapply ex_ir in IHA2 ; [ | apply Permutation_Type_swap ].
+  apply (neg_plus_propag _ _ _ _ IHA1) in IHA2.
+  eapply ex_ir ; [ | apply Permutation_Type_swap ].
   apply negR_ilr...
   apply negR_irr.
   cons2app.
   rewrite <- (app_nil_l _).
   eapply cut_ir ; [ | | apply IHA2 ]...
-  rewrite <- (app_nil_l _).
-  apply plus_ilr.
-  + list_simpl.
-    apply plus_irr1...
-  + list_simpl.
-    apply plus_irr2...
-- eexists.
-  apply negR_ilr...
+- apply negR_ilr...
   apply negR_irr.
-  eapply ex_ir ; [ | apply perm_swap ].
+  eapply ex_ir ; [ | apply Permutation_Type_swap ].
   apply negR_ilr...
   change (ioc (negR (trans A)) :: nil)
     with (map ioc (negR (trans A) :: nil)).
@@ -318,12 +255,11 @@ induction A ;
   rewrite <- (app_nil_l _).
   apply de_ilr.
   apply negR_irr.
-  eapply ex_ir ; [ | apply perm_swap ]...
-- eexists.
-  eapply ex_ir ; [ | apply perm_swap ].
+  eapply ex_ir ; [ | apply Permutation_Type_swap ]...
+- eapply ex_ir ; [ | apply Permutation_Type_swap ].
   apply negR_ilr...
   apply negR_irr.
-  eapply ex_ir ; [ | apply perm_swap ].
+  eapply ex_ir ; [ | apply Permutation_Type_swap ].
   apply negR_ilr...
   change (ioc (negR (trans (dual A))) :: nil)
     with (map ioc (negR (trans (dual A)) :: nil)).
@@ -334,26 +270,17 @@ induction A ;
 Qed.
 
 Lemma trans_subs : forall A B x,
-  (isubs (negR (trans B)) (a2i x) R = R) -> exists s,
+  (isubs (negR (trans B)) (a2i x) R = R) ->
   ill_ll (isubs (negR (trans B)) (a2i x) (trans A)
-              :: negR (trans (subs B x A)):: nil) R s.
-Proof with myeeasy.
+              :: negR (trans (subs B x A)):: nil) R.
+Proof with myeeasy ; try now (apply ax_exp_ill).
 intros A B x HR.
-induction A ;
-  destruct (@ax_exp_ill ipfrag_ill R) as [sR axR] ;
-  destruct (@ax_exp_ill ipfrag_ill (trans B)) as [sB axB] ;
-  try destruct IHA as [s0 IHA] ;
-  try destruct IHA1 as [s1 IHA1] ;
-  try destruct IHA2 as [s2 IHA2] ;
-  simpl ; try rewrite HR.
-- case_eq (ateq a x) ; intros Hateq ; eexists.
+induction A ; simpl ; try rewrite HR.
+- case_eq (ateq a x) ; intros Hateq.
   + unfold repl_at ; rewrite Hateq ; simpl.
     assert (iateq (a2i a) (a2i x) = true) as Hiateq
       by (rewrite <- ateq_a2i ; assumption).
     unfold repl_iat ; rewrite Hiateq ; simpl.
-    apply negR_ilr...
-    apply negR_irr.
-    eapply ex_ir ; [ | apply perm_swap ].
     apply negR_ilr...
   + case_eq (iateq (a2i a) (a2i x)) ; intros Hiateq.
     * exfalso.
@@ -363,12 +290,8 @@ induction A ;
       inversion Hateq.
     * unfold repl_at ; rewrite Hateq ; simpl.
       unfold repl_iat ; rewrite Hiateq ; simpl.
-      eapply ex_ir ; [ | apply perm_swap ].
+      eapply ex_ir ; [ | apply Permutation_Type_swap ].
       apply negR_ilr...
-      apply negR_irr.
-      eapply ex_ir ; [ | apply perm_swap ].
-      apply negR_ilr...
-      apply ax_ir.
 - case_eq (ateq a x) ; intros Hateq.
   + unfold repl_at ; rewrite Hateq ; simpl.
     assert (iateq (a2i a) (a2i x) = true) as Hiateq
@@ -383,50 +306,30 @@ induction A ;
       inversion Hateq.
     * unfold repl_at ; rewrite Hateq ; simpl.
       unfold repl_iat ; rewrite Hiateq ; simpl.
-      eexists.
-      eapply ex_ir ; [ | apply perm_swap ].
+      eapply ex_ir ; [ | apply Permutation_Type_swap ].
       apply negR_ilr...
-      apply ax_ir.
-- eexists.
-  eapply ex_ir ; [ | apply perm_swap ].
+- eapply ex_ir ; [ | apply Permutation_Type_swap ].
+  apply negR_ilr...
+- eapply ex_ir ; [ | apply Permutation_Type_swap ].
+  apply negR_ilr...
+- eapply ex_ir ; [ | apply Permutation_Type_swap ].
   apply negR_ilr...
   apply negR_irr.
-  eapply ex_ir ; [ | apply perm_swap ].
-  apply negR_ilr...
-  rewrite <- (app_nil_l _).
-  apply one_ilr.
-  apply one_irr.
-- eexists.
-  eapply ex_ir ; [ | apply perm_swap ].
-  apply negR_ilr...
-  rewrite <- (app_nil_l _).
-  apply one_ilr.
-  apply one_irr.
-- eexists.
-  eapply ex_ir ; [ | apply perm_swap ].
-  apply negR_ilr...
-  apply negR_irr.
-  eapply ex_ir ; [ | apply perm_swap ].
+  eapply ex_ir ; [ | apply Permutation_Type_swap ].
   apply negR_ilr...
   rewrite <- (app_nil_l _).
   apply tens_ilr.
   list_simpl ; cons2app.
   apply tens_irr ; apply negR_irr...
 - eapply neg_tens_propag...
-- eexists.
-  eapply ex_ir ; [ | apply perm_swap ].
+- eapply ex_ir ; [ | apply Permutation_Type_swap ].
   apply negR_ilr...
-  apply negR_irr.
-  rewrite <- (app_nil_l _).
-  apply zero_ilr...
-- eexists.
-  rewrite <- (app_nil_l _).
+- rewrite <- (app_nil_l _).
   apply zero_ilr.
-- eexists.
-  eapply ex_ir ; [ | apply perm_swap ].
+- eapply ex_ir ; [ | apply Permutation_Type_swap ].
   apply negR_ilr...
   apply negR_irr.
-  eapply ex_ir ; [ | apply perm_swap ].
+  eapply ex_ir ; [ | apply Permutation_Type_swap ].
   apply negR_ilr...
   rewrite <- (app_nil_l _).
   apply plus_ilr ; list_simpl.
@@ -435,11 +338,10 @@ induction A ;
   + apply plus_irr2.
     apply negR_irr...
 - eapply neg_plus_propag...
-- eexists.
-  eapply ex_ir ; [ | apply perm_swap ].
+- eapply ex_ir ; [ | apply Permutation_Type_swap ].
   apply negR_ilr...
   apply negR_irr.
-  eapply ex_ir ; [ | apply perm_swap ].
+  eapply ex_ir ; [ | apply Permutation_Type_swap ].
   apply negR_ilr...
   change (ioc (negR (trans (subs B x A))) :: nil)
     with (map ioc (negR (trans (subs B x A)) :: nil)).
@@ -447,8 +349,7 @@ induction A ;
   rewrite <- (app_nil_l _).
   apply de_ilr.
   apply negR_irr...
-- eexists.
-  eapply ex_ir ; [ | apply perm_swap ].
+- eapply ex_ir ; [ | apply Permutation_Type_swap ].
   apply negR_ilr...
   change (ioc (ilmap (ilmap (isubs (negR (trans B)) (a2i x) (trans A)) R) R) :: nil)
     with (map ioc (negR (negR (isubs (negR (trans B)) (a2i x) (trans A))) :: nil)).
@@ -457,7 +358,7 @@ induction A ;
   apply de_ilr.
   apply negR_irr.
   list_simpl.
-  eapply ex_ir ; [ | apply perm_swap ].
+  eapply ex_ir ; [ | apply Permutation_Type_swap ].
   apply negR_ilr...
   apply negR_irr...
 Qed.
@@ -468,135 +369,121 @@ Qed.
 (** The translation maps [ll] proofs into [ill] proofs
 (under some conditions for [mix0] and [mix2]). **)
 
-Lemma ll_to_ill_trans_gen : forall l l0 s,
-  (pmix0 P = true -> exists s0, ill_ll (map ioc l0) R s0) ->
-  (pmix2 P = true -> forall l1 l2 s1 s2,
-    ill_ll (map ioc l0 ++ map trans l1) R s1 ->
-    ill_ll (map ioc l0 ++ map trans l2) R s2 ->
-      exists s0, ill_ll (map ioc l0 ++ map trans l2 ++ map trans l1) R s0) ->
-  ll P l s -> exists s', ill_ll (map ioc l0 ++ map trans l) R s'.
-Proof with myeeasy ; try PEperm_solve.
-intros l l0 s Hmix0 Hmix2 Hll.
-destruct (@ax_exp_ill ipfrag_ill R) as [sax Hax].
+Lemma ll_to_ill_trans_gen : forall l l0,
+  (pmix0 P = true -> ill_ll (map ioc l0) R) ->
+  (pmix2 P = true -> forall l1 l2,
+    ill_ll (map ioc l0 ++ map trans l1) R ->
+    ill_ll (map ioc l0 ++ map trans l2) R ->
+      ill_ll (map ioc l0 ++ map trans l2 ++ map trans l1) R) ->
+  ll P l -> ill_ll (map ioc l0 ++ map trans l) R.
+Proof with myeeasy ; (try now (apply ax_exp_ill)) ; try PEperm_Type_solve.
+intros l l0 Hmix0 Hmix2 Hll.
+assert (Hax := @ax_exp_ill ipfrag_ill R).
 rewrite <- (app_nil_l (R :: _)) in Hax.
-assert (Hax' := wk_list_ilr l0 _ _ _ _ Hax).
-destruct Hax' as [sax' Hax'].
+assert (ill ipfrag_ill (nil ++ map ioc l0 ++ R :: nil) R) as Hax'.
+{ apply wk_list_ilr.
+  apply ax_exp_ill. }
 rewrite <- (app_nil_r (map _ _)) in Hmix0.
 induction Hll ; 
-  try (destruct IHHll as [s' pi']) ;
-  try (destruct IHHll1 as [s1' pi1']) ;
-  try (destruct IHHll2 as [s2' pi2']) ;
-  try (apply Hmix0 ; myeasy ; fail) ;
-  try (rewrite map_app ; eapply Hmix2 ; myeeasy ; fail) ;
-  try (apply P_axfree in H ; inversion H ; fail) ;
-  try (inversion f ; fail) ;
+  (try now (apply Hmix0)) ;
+  (try now (rewrite map_app ; eapply Hmix2)) ;
+  (try now (apply P_axfree in H ; inversion H)) ;
+  (try now (inversion f)) ;
   simpl.
-- eexists.
-  eapply ex_ir.
+- eapply ex_ir.
   + eapply lmap_ilr ; [ | apply Hax' ].
     eapply (ax_ir _ (a2i X)).
-  + PEperm_solve.
-- eexists.
-  simpl in H.
-  rewrite P_perm in H.
+  + PEperm_Type_solve.
+- simpl in p.
+  rewrite P_perm in p.
   eapply ex_ir...
-  apply PEperm_app_head...
-  apply Permutation_map...
-- eexists.
-  eapply ex_ir ; [ | apply Permutation_middle ].
+  apply PEperm_Type_app_head...
+  apply Permutation_Type_map...
+- eapply ex_ir ; [ | apply Permutation_Type_middle ].
   rewrite <- (app_nil_l _).
   rewrite <- (app_nil_l _).
   apply lmap_ilr...
   + apply one_irr.
   + eapply ex_ir...
-- eexists.
-  apply one_ilr...
+- apply one_ilr...
 - apply (ex_ir _ _ (trans A :: map ioc l0 ++ map trans l1))
-    in pi1'...
-  apply negR_irr in pi1'.
+    in IHHll1...
+  apply negR_irr in IHHll1.
   apply (ex_ir _ _ (trans B :: map ioc l0 ++ map trans l2))
-    in pi2'...
-  apply negR_irr in pi2'.
-  apply (tens_irr _ _ _ _ _ _ _ pi1') in pi2'.
-  apply (lmap_ilr _ _ _ _ _ _ _ _ _ pi2') in Hax.
+    in IHHll2...
+  apply negR_irr in IHHll2.
+  apply (tens_irr _ _ _ _ _ IHHll1) in IHHll2.
+  apply (lmap_ilr _ _ _ _ _ _ _ IHHll2) in Hax.
   rewrite <- (app_nil_l (map _ _ ++ _)).
   change nil with (map ioc nil).
   rewrite <- (app_nil_l (map _ _)).
   rewrite <- app_assoc.
   eapply co_list_ilr.
-  apply (ex_ir _ _ _ _ _ Hax)...
-- eexists.
-  apply tens_ilr...
-- eexists.
-  apply zero_ilr.
-- eexists.
-  apply (ex_ir _ _ (trans A :: map ioc l0 ++ map trans l))
-    in pi'...
-  apply negR_irr in pi'.
-  apply (plus_irr1 _ _ (negR (trans B))) in pi'.
-  apply (lmap_ilr _ _ _ _ _ _ _ _ _ pi') in Hax.
-  apply (ex_ir _ _ _ _ _ Hax)...
-- eexists.
-  apply (ex_ir _ _ (trans A :: map ioc l0 ++ map trans l))
-    in pi'...
-  apply negR_irr in pi'.
-  apply (plus_irr2 _ _ (negR (trans B))) in pi'.
-  apply (lmap_ilr _ _ _ _ _ _ _ _ _ pi') in Hax.
-  apply (ex_ir _ _ _ _ _ Hax)...
-- eexists.
-  apply plus_ilr...
-- eexists.
-  simpl in pi' ; rewrite map_map in pi'.
-  simpl in pi' ; rewrite <- map_map in pi'.
+  apply (ex_ir _ _ _ _ Hax)...
+- apply tens_ilr...
+- apply zero_ilr.
+- apply (ex_ir _ _ (trans A :: map ioc l0 ++ map trans l))
+    in IHHll...
+  apply negR_irr in IHHll.
+  apply (plus_irr1 _ _ (negR (trans B))) in IHHll.
+  apply (lmap_ilr _ _ _ _ _ _ _ IHHll) in Hax.
+  apply (ex_ir _ _ _ _ Hax)...
+- apply (ex_ir _ _ (trans A :: map ioc l0 ++ map trans l))
+    in IHHll...
+  apply negR_irr in IHHll.
+  apply (plus_irr2 _ _ (negR (trans B))) in IHHll.
+  apply (lmap_ilr _ _ _ _ _ _ _ IHHll) in Hax.
+  apply (ex_ir _ _ _ _ Hax)...
+- apply plus_ilr...
+- simpl in IHHll ; rewrite map_map in IHHll.
+  simpl in IHHll ; rewrite <- map_map in IHHll.
   apply (ex_ir _ _ (trans A :: map ioc (l0 ++ map (fun x => (negR (negR (trans x)))) l)))
-    in pi'...
-  + apply negR_irr in pi'.
-    apply oc_irr in pi'.
-    eapply ex_ir ; [ | apply Permutation_middle ].
+    in IHHll...
+  + apply negR_irr in IHHll.
+    apply oc_irr in IHHll.
+    eapply ex_ir ; [ | apply Permutation_Type_middle ].
     apply negR_ilr...
     eapply ex_ir...
     list_simpl...
     rewrite ? map_map...
   + list_simpl...
     rewrite ? map_map...
-- eexists.
-  apply de_ilr...
-  eapply ex_ir ; [ | apply Permutation_middle ].
+- apply de_ilr...
+  eapply ex_ir ; [ | apply Permutation_Type_middle ].
   apply negR_ilr...
   apply negR_irr.
   eapply ex_ir...
-- eexists.
-  apply wk_ilr...
-- eexists.
-  rewrite <- (app_nil_l (map _ _ ++ _)).
+- apply wk_ilr...
+- rewrite <- (app_nil_l (map _ _ ++ _)).
   apply co_ilr.
   eapply ex_ir...
-- apply (ex_ir _ _ (trans (dual A) :: map ioc l0 ++ map trans l1)) in pi1'...
-  apply negR_irr in pi1'.
-  apply (ex_ir _ _ (trans A :: map ioc l0 ++ map trans l2)) in pi2'...
-  apply negR_irr in pi2'.
-  destruct (trans_dual A) as [s0 pi0].
+- apply (ex_ir _ _ (trans (dual A) :: map ioc l0 ++ map trans l1)) in IHHll1...
+  apply negR_irr in IHHll1.
+  apply (ex_ir _ _ (trans A :: map ioc l0 ++ map trans l2)) in IHHll2...
+  apply negR_irr in IHHll2.
+  assert (pi0 := trans_dual A).
   rewrite <- (app_nil_l _) in pi0.
-  eapply (cut_ir _ _ _ _ _ _ _ _ pi2') in pi0.
+  eapply (cut_ir _ _ _ _ _ _ IHHll2) in pi0.
   list_simpl in pi0 ; rewrite app_assoc in pi0.
-  eapply (cut_ir _ _ _ _ _ _ _ _ pi1') in pi0.
+  eapply (cut_ir _ _ _ _ _ _ IHHll1) in pi0.
   change (map ioc l0) with (map ioc nil ++ map ioc l0).
   rewrite <- (app_nil_l (map ioc nil)).
   rewrite <- ? app_assoc.
   eapply co_list_ilr.
   eapply ex_ir...
+- intuition.
 Unshelve. all : reflexivity.
 Qed.
 
-Theorem ll_to_ill_trans : forall l s,
-  (pmix0 P = true -> exists s0, ill_ll nil R s0) ->
-  (pmix2 P = true -> forall l1 l2 s1 s2,
-    ill_ll (map trans l1) R s1 ->
-    ill_ll (map trans l2) R s2 ->
-    exists s0, ill_ll (map trans l2 ++ map trans l1) R s0) ->
-      ll P l s -> exists s', ill_ll (map trans l) R s'.
+Theorem ll_to_ill_trans : forall l,
+  (pmix0 P = true -> ill_ll nil R) ->
+  (pmix2 P = true -> forall l1 l2,
+    ill_ll (map trans l1) R ->
+    ill_ll (map trans l2) R ->
+      ill_ll (map trans l2 ++ map trans l1) R) ->
+      ll P l -> ill_ll (map trans l) R.
 Proof with myeeasy.
-intros l s Hmix0 Hmix2 Hll.
+intros l Hmix0 Hmix2 Hll.
 rewrite <- (app_nil_l (map _ _)).
 change nil with (map ioc nil).
 eapply ll_to_ill_trans_gen...
@@ -605,38 +492,26 @@ Qed.
 
 (** In [llR] (where [bot] is equivalent to [R]),
   [A] is implied by the dual of its translation. *)
-Lemma back_to_llR : forall A, exists s,
-  llR (unill R) (unill (trans A) :: A :: nil) s.
-Proof with myeeasy ; try ((try rewrite a2a_i) ; PCperm_solve).
-induction A ; simpl ; 
-  try (destruct IHA as [s IHA]) ;
-  try (destruct IHA1 as [s1 IHA1]) ;
-  try (destruct IHA2 as [s2 IHA2]) ;
-  rewrite ? bidual.
-- eexists.
-  apply parr_r.
+Lemma back_to_llR : forall A,
+  llR (unill R) (unill (trans A) :: A :: nil).
+Proof with myeeasy ; try ((try rewrite a2a_i) ; PCperm_Type_solve).
+induction A ; simpl ; rewrite ? bidual.
+- apply parr_r.
   apply (ex_r _ ((covar a :: var a :: nil) ++ unill R :: nil))...
   eapply (@cut_r (pfrag_llR (unill R)) eq_refl (dual one)).
   + apply (ex_r _ (unill R :: one :: nil))...
-    apply gax_r.
-    right...
+    apply (gax_r (pfrag_llR (unill R)) false).
   + apply bot_r.
     apply ax_r.
-- eexists.
-  apply (ex_r _ (covar a :: var a :: nil))...
+- apply (ex_r _ (covar a :: var a :: nil))...
   apply ax_r...
-- eexists.
-  eapply parr_r.
+- eapply parr_r.
   apply (bot_r (pfrag_llR (unill R))).
-  apply gax_r.
-  right...
-- eexists.
-  apply (ex_r _ (bot :: one :: nil))...
+  apply (gax_r (pfrag_llR (unill R)) false).
+- apply (ex_r _ (bot :: one :: nil))...
   apply bot_r.
   apply one_r.
 - assert (Hax := @ax_exp (pfrag_llR (unill R)) (unill R)).
-  destruct Hax as [sax Hax].
-  eexists.
   apply parr_r.
   apply parr_r.
   change (tens (dual (unill R)) (unill (trans A2)) ::
@@ -644,78 +519,65 @@ induction A ; simpl ;
     with (tens (dual (unill R)) (unill (trans A2)) ::  
     (tens (dual (unill R)) (unill (trans A1)) :: unill R :: tens A1 A2 :: nil) ++ nil).
   apply tens_r.
-  + apply gax_r.
-    left...
+  + apply (gax_r (pfrag_llR (unill R)) true).
   + apply (ex_r _ (tens (dual (unill R)) (unill (trans A1))
              :: (unill (trans A2) :: tens A1 A2 :: nil) ++ (unill R :: nil)))...
     apply tens_r.
-    -- eapply ex_r ; [ | apply perm_swap ]...
+    -- eapply ex_r ; [ | apply Permutation_Type_swap ]...
     -- apply (ex_r _ (tens A1 A2 ::
              (unill (trans A2) :: nil) ++ unill (trans A1) :: nil))...
        apply tens_r.
        ++ eapply ex_r ; [ apply IHA1 | ]...
        ++ eapply ex_r ; [ apply IHA2 | ]...
-- eexists.
-  apply (ex_r _ (parr A1 A2 ::
+- apply (ex_r _ (parr A1 A2 ::
                  tens (unill (trans A1)) (unill (trans A2)) :: nil))...
   apply parr_r.
   apply (ex_r _ (tens (unill (trans A1)) (unill (trans A2))
                   :: (A2 :: nil) ++ (A1 :: nil)))...
   apply tens_r...
-- eexists.
-  apply parr_r.
+- apply parr_r.
   apply top_r.
-- eexists.
-  eapply ex_r ; [ | apply perm_swap ].
+- eapply ex_r ; [ | apply Permutation_Type_swap ].
   eapply top_r.
 - assert (Hax := @ax_exp (pfrag_llR (unill R)) (unill R)).
-  destruct Hax as [sax Hax].
-  eexists.
   apply parr_r.
   apply with_r.
   + apply (ex_r _ (tens (dual (unill R)) (unill (trans A1)) ::
                     (aplus A1 A2 :: nil) ++ unill R :: nil))...
     apply tens_r.
-    * eapply ex_r ; [ | apply perm_swap ]...
-    * eapply ex_r ; [ | apply perm_swap ].
+    * eapply ex_r ; [ | apply Permutation_Type_swap ]...
+    * eapply ex_r ; [ | apply Permutation_Type_swap ].
       apply plus_r1.
-      eapply ex_r ; [ | apply perm_swap ]...
+      eapply ex_r ; [ | apply Permutation_Type_swap ]...
   + apply (ex_r _ (tens (dual (unill R)) (unill (trans A2)) ::
                     (aplus A1 A2 :: nil) ++ unill R :: nil))...
     apply tens_r...
-    * eapply ex_r ; [ | apply perm_swap ]...
-    * eapply ex_r ; [ | apply perm_swap ].
+    * eapply ex_r ; [ | apply Permutation_Type_swap ]...
+    * eapply ex_r ; [ | apply Permutation_Type_swap ].
       apply plus_r2.
-      eapply ex_r ; [ | apply perm_swap ]...
+      eapply ex_r ; [ | apply Permutation_Type_swap ]...
 - assert (Hax := @ax_exp (pfrag_llR (unill R)) (unill R)).
-  destruct Hax as [sax Hax].
-  eexists.
-  eapply ex_r ; [ | apply perm_swap ].
+  eapply ex_r ; [ | apply Permutation_Type_swap ].
   apply with_r.
-  + eapply ex_r ; [ | apply perm_swap ].
+  + eapply ex_r ; [ | apply Permutation_Type_swap ].
     apply plus_r1...
-  + eapply ex_r ; [ | apply perm_swap ].
+  + eapply ex_r ; [ | apply Permutation_Type_swap ].
     apply plus_r2...
-- eexists.
-  apply parr_r.
+- apply parr_r.
   apply (ex_r _ ((oc A ::
                   map wn (tens (dual (unill R)) (unill (trans A)) :: nil))
                   ++ unill R :: nil)) ; [idtac | simpl]...
   apply (@cut_r (pfrag_llR (unill R)) eq_refl (dual one)).
   + apply (ex_r _ (unill R :: one :: nil))...
-    apply gax_r.
-    right...
+    apply (gax_r (pfrag_llR (unill R)) false).
   + apply bot_r.
     apply oc_r ; simpl.
     apply (ex_r _ ((wn (tens (dual (unill R)) (unill (trans A))) :: nil)
                      ++ (A :: nil) ++ nil))...
     apply de_r.
     apply tens_r...
-    apply gax_r.
-    left...
+    apply (gax_r (pfrag_llR (unill R)) true).
 - assert (Hax := @ax_exp (pfrag_llR (unill R)) (unill R)).
-  destruct Hax as [sax Hax].
-  eexists.
   change (wn A :: nil) with (map wn (A :: nil)).
   apply oc_r ; simpl.
   apply parr_r.
@@ -724,64 +586,51 @@ induction A ; simpl ;
   + eapply ex_r...
   + apply (ex_r _ (wn A :: unill (trans A) :: nil))...
     apply de_r...
-    eapply ex_r ; [ | apply perm_swap ]...
+    eapply ex_r ; [ | apply Permutation_Type_swap ]...
 Qed.
 
 (** The previous lemma comes with the following result from the [ll_fragments] library:
 <<
-Lemma ll_to_llR : forall R l s, ll_ll l s -> exists s', llR R l s'.
+Lemma ll_to_llR : forall R l, ll_ll l -> llR R l.
 >> to deduce: *)
 
 (** A sequent whose translation is provable in [ill] was provable in [llR]. *)
-Lemma ill_trans_to_llR : forall l s,
-  ill_ll (map trans l) R s -> exists s', llR (unill R) l s'.
-Proof with myeeasy ; try PCperm_solve.
-intros l s Hill.
+Lemma ill_trans_to_llR : forall l,  ill_ll (map trans l) R -> llR (unill R) l.
+Proof with myeeasy ; try PCperm_Type_solve.
+intros l Hill.
 apply (ill_to_ll i2a) in Hill.
-clear s ; destruct Hill as [s Hill].
-apply (stronger_pfrag _ (mk_pfrag true (fun _ => False) false false true))
+apply (stronger_pfrag _ (mk_pfrag true NoAxioms false false true))
   in Hill.
 - eapply cut_admissible_axfree in Hill.
-  + clear s ; destruct Hill as [s Hill].
-    apply (ll_to_llR (unill R)) in Hill.
-    clear s ; destruct Hill as [s Hill].
-    assert (forall l' s',
-      llR (unill R) (l' ++ map dual (map unill (map trans (rev l)))) s'
-        -> exists s'', llR (unill R) (l' ++ rev l) s'') as Hll.
+  + apply (ll_to_llR (unill R)) in Hill.
+    assert (forall l',
+      llR (unill R) (l' ++ map dual (map unill (map trans (rev l))))
+        -> llR (unill R) (l' ++ rev l)) as Hll.
     { clear.
-      induction l using rev_ind ; intros...
-      - eexists...
-      - assert (Hb := back_to_llR x).
-        destruct Hb as [sb Hb].
-        rewrite rev_unit in H.
-       apply (ex_r _ _ (dual (unill (trans x))
-                 :: l' ++ map dual (map unill (map trans (rev l))))) in H...
-        apply (@cut_r _ (eq_refl (pcut (pfrag_llR (unill R)))) _ _ _ _ _ H) in Hb.
-        rewrite rev_unit.
-        change (x :: rev l) with ((x :: nil) ++ rev l).
-        rewrite app_assoc.
-        eapply IHl.
-        eapply ex_r... }
-    assert (exists s, llR (unill R) (dual (unill R) :: nil) s) as [sR HR].
-    { eexists.
-      apply gax_r.
-      left... }
-    apply (@cut_r _ (eq_refl (pcut (pfrag_llR (unill R)))) _ _ _ _ _ HR) in Hill.
+      induction l using rev_ind_Type ; intros...
+      assert (Hb := back_to_llR x).
+      rewrite rev_unit in X.
+      apply (ex_r _ _ (dual (unill (trans x))
+               :: l' ++ map dual (map unill (map trans (rev l))))) in X...
+      apply (@cut_r _ (eq_refl (pcut (pfrag_llR (unill R)))) _ _ _ X) in Hb.
+      rewrite rev_unit.
+      change (x :: rev l) with ((x :: nil) ++ rev l).
+      rewrite app_assoc.
+      eapply IHl.
+      eapply ex_r... }
+    assert (llR (unill R) (dual (unill R) :: nil)) as HR
+      by (apply (gax_r (pfrag_llR (unill R)) true)).
+    apply (@cut_r _ (eq_refl (pcut (pfrag_llR (unill R)))) _ _ _ HR) in Hill.
     rewrite app_nil_r in Hill.
     rewrite <- (app_nil_l (rev _)) in Hill.
     rewrite <- ? map_rev in Hill.
     apply Hll in Hill.
-    destruct Hill as [s' Hill].
-    eexists.
     eapply ex_r ; [ apply Hill | ].
     symmetry.
-    apply Permutation_rev.
-  + intros f Hax.
-    apply Hax.
+    apply Permutation_Type_rev.
+  + intros Hax ; inversion Hax.
 - nsplit 5 ; myeasy.
-  intros f Hax.
-  destruct Hax as (l0 & C & _ & Hax).
-  inversion Hax.
+  intros Hax ; inversion Hax.
 Qed.
 
 
@@ -790,7 +639,7 @@ Qed.
 extension of [ll_to_ill_trans] *)
 
 (** Elementary intuitionistic formulas *)
-Inductive ielem : iformula -> Prop :=
+Inductive ielem : iformula -> Type :=
 | ie_ivar : forall X, X <> atN -> ielem (ivar X)
 | ie_ione : ielem ione
 | ie_itens : forall A B, ielem A -> ielem B -> ielem (itens A B)
@@ -798,213 +647,163 @@ Inductive ielem : iformula -> Prop :=
 | ie_iplus : forall A B, ielem A -> ielem B -> ielem (iplus A B)
 | ie_itop : ielem itop.
 
-Lemma ie_ie : forall A, ielem A -> exists s,
-  ill_ll (A :: nil) (negR (trans (unill A))) s.
-Proof.
-destruct (@ax_exp_ill ipfrag_ill R) as [sR HaxR].
+Lemma ie_ie : forall A, ielem A ->
+  ill_ll (A :: nil) (negR (trans (unill A))).
+Proof with try now (apply ax_exp_ill).
 induction A ; intros Hgfn ; inversion Hgfn ;
   simpl ; unfold trans.
-- eexists.
-  unfold a2i ; unfold i2a ; rewrite (i2i_not_atN _ H0).
+- unfold a2i ; unfold i2a ; rewrite (i2i_not_atN _ H0).
   apply negR_irr.
-  apply negR_ilr.
-  + eassumption.
-  + apply ax_ir.
-- destruct (@ax_exp_ill ipfrag_ill ione) as [s1 Hax1].
-  eexists.
-  apply negR_irr.
-  apply negR_ilr ; eassumption.
+  apply negR_ilr...
+- apply negR_irr.
+  apply negR_ilr...
 - apply IHA1 in H1.
   apply IHA2 in H2.
-  destruct H1 as [s1 H1].
-  destruct H2 as [s2 H2].
-  eexists.
   apply negR_irr.
-  apply negR_ilr.
-  + eassumption.
-  + rewrite <- (app_nil_l _).
-    apply tens_ilr.
-    list_simpl ; cons2app.
-    apply tens_irr ; eassumption.
-- destruct (@ax_exp_ill ipfrag_ill ione) as [s1 Hax1].
-  eexists.
-  apply negR_irr.
+  apply negR_ilr...
+  rewrite <- (app_nil_l _).
+  apply tens_ilr.
+  list_simpl ; cons2app.
+  apply tens_irr ; eassumption.
+- apply negR_irr.
   rewrite <- (app_nil_l _).
   apply zero_ilr.
-- destruct (@ax_exp_ill ipfrag_ill ione) as [s1 Hax1].
-  eexists.
-  rewrite <- (app_nil_l _).
+- rewrite <- (app_nil_l _).
   apply zero_ilr.
 - apply IHA1 in H1.
   apply IHA2 in H2.
-  destruct H1 as [s1 H1].
-  destruct H2 as [s2 H2].
-  eexists.
   apply negR_irr.
-  apply negR_ilr.
-  + eassumption.
-  + rewrite <- (app_nil_l _).
-    apply plus_ilr ; constructor ; eassumption.
+  apply negR_ilr...
+  rewrite <- (app_nil_l _).
+  apply plus_ilr ; constructor ; eassumption.
 Qed.
 
-Lemma ie_dual : forall A, ielem A -> exists s,
-  ill_ll (trans (dual (unill A)) :: nil) A s.
-Proof.
-destruct (@ax_exp_ill ipfrag_ill R) as [sR HaxR].
+Lemma ie_dual : forall A, ielem A ->
+  ill_ll (trans (dual (unill A)) :: nil) A.
+Proof with try now (apply ax_exp_ill).
 induction A ; intros Hgfn ; inversion Hgfn ;
-  simpl ; unfold trans.
-- eexists.
-  unfold a2i ; unfold i2a ; rewrite (i2i_not_atN _ H0).
-  apply ax_ir.
-- apply ax_exp_ill.
+  simpl ; unfold trans...
+- unfold a2i ; unfold i2a ; rewrite (i2i_not_atN _ H0)...
 - apply IHA1 in H1.
   apply IHA2 in H2.
-  destruct H1 as [s1 H1].
-  destruct H2 as [s2 H2].
-  eexists.
   rewrite <- (app_nil_l _).
   apply tens_ilr.
   list_simpl.
-  eapply ex_ir ; [ | apply perm_swap ].
+  eapply ex_ir ; [ | apply Permutation_Type_swap ].
   cons2app.
   apply tens_irr ; eassumption.
-- eexists ; apply top_irr.
-- eexists ; rewrite <- (app_nil_l _) ; apply zero_ilr.
+- apply top_irr.
 - apply IHA1 in H1.
   apply IHA2 in H2.
-  destruct H1 as [s1 H1].
-  destruct H2 as [s2 H2].
-  eexists.
   rewrite <- (app_nil_l _).
   apply plus_ilr ; constructor ; eassumption.
 Qed.
 
 End RTranslation.
 
-Lemma ie_ie_diag : forall A, ielem A -> exists s,
-  ill_ll (trans A (unill A) :: A :: nil) A s.
+Lemma ie_ie_diag : forall A, ielem A ->
+  ill_ll (trans A (unill A) :: A :: nil) A.
 Proof.
 intros A Hgfn.
-destruct (ie_ie A _ Hgfn) as [s H].
-destruct (@ax_exp_ill ipfrag_ill A) as [sA HaxA].
-destruct (@ax_exp_ill ipfrag_ill (trans A (unill A))) as [sA' HaxA'].
-eexists.
-eapply ex_ir ; [ | apply perm_swap ].
+eapply ex_ir ; [ | apply Permutation_Type_swap ].
 cons2app.
 rewrite <- (app_nil_l _).
 eapply cut_ir.
 - reflexivity.
-- apply H.
-- apply negR_ilr ; eassumption.
+- apply ie_ie.
+  assumption.
+- apply negR_ilr ; apply ax_exp_ill.
 Qed.
 
-Lemma ie_dual_diag : forall A, ielem A -> exists s,
-  ill_ll (trans A (dual (unill A)) :: nil) A s.
+Lemma ie_dual_diag : forall A, ielem A ->
+  ill_ll (trans A (dual (unill A)) :: nil) A.
 Proof.
 intros A.
 apply ie_dual.
 Qed.
 
-Proposition llR_ie_to_ill_trans : forall R l s, ielem R ->
-  llR (unill R) l s -> exists s', ill_ll (map (trans R) l) R s'.
-Proof with myeeasy ; try PEperm_solve.
-intros R l s Hie Hll.
-destruct (@ax_exp_ill ipfrag_ill R) as [sax Hax].
+Proposition llR_ie_to_ill_trans : forall R l, ielem R ->
+  llR (unill R) l -> ill_ll (map (trans R) l) R.
+Proof with myeeasy ; try PEperm_Type_solve.
+intros R l Hie Hll.
+assert (Hax := @ax_exp_ill ipfrag_ill R).
 rewrite <- (app_nil_l (R :: _)) in Hax.
 induction Hll ; 
-  try (destruct IHHll as [s' pi']) ;
-  try (destruct IHHll1 as [s1' pi1']) ;
-  try (destruct IHHll2 as [s2' pi2']) ;
-  try (apply Hmix0 ; myeasy ; fail) ;
-  try (rewrite map_app ; eapply Hmix2 ; myeeasy ; fail) ;
-  try (apply P_axfree in H ; inversion H ; fail) ;
-  try (inversion f ; fail) ;
+  (try now (apply Hmix0)) ;
+  (try now (rewrite map_app ; eapply Hmix2)) ;
+  (try now (apply P_axfree in H ; inversion H)) ;
+  (try now (inversion f)) ;
   simpl.
-- eexists.
-  eapply ex_ir.
+- eapply ex_ir.
   + eapply lmap_ilr ; [ | apply Hax ].
     eapply (ax_ir _ (a2i X)).
-  + PEperm_solve.
-- eexists.
-  eapply ex_ir...
-  apply Permutation_map...
-- eexists.
-  rewrite <- (app_nil_l _).
+  + PEperm_Type_solve.
+- eapply ex_ir...
+  apply Permutation_Type_map...
+- rewrite <- (app_nil_l _).
   rewrite <- (app_nil_l _).
   apply lmap_ilr...
   apply one_irr.
-- eexists.
-  rewrite <- (app_nil_l (ione :: _)).
+- rewrite <- (app_nil_l (ione :: _)).
   apply one_ilr...
-- apply negR_irr in pi1'.
-  apply negR_irr in pi2'.
-  apply (tens_irr _ _ _ _ _ _ _ pi1') in pi2'.
-  apply (lmap_ilr _ _ _ _ _ _ _ _ _ pi2') in Hax.
-  eexists.
-  apply (ex_ir _ _ _ _ _ Hax)...
-- eexists.
-  rewrite <- (app_nil_l (itens _ _ :: _)).
+- apply negR_irr in IHHll1.
+  apply negR_irr in IHHll2.
+  apply (tens_irr _ _ _ _ _ IHHll1) in IHHll2.
+  apply (lmap_ilr _ _ _ _ _ _ _ IHHll2) in Hax.
+  apply (ex_ir _ _ _ _ Hax)...
+- rewrite <- (app_nil_l (itens _ _ :: _)).
   apply tens_ilr...
-- eexists.
-  rewrite <- (app_nil_l (izero :: _)).
+- rewrite <- (app_nil_l (izero :: _)).
   apply zero_ilr.
-- eexists.
-  apply negR_irr in pi'.
-  apply (plus_irr1 _ _ (negR R (trans R B))) in pi'.
-  apply (lmap_ilr _ _ _ _ _ _ _ _ _ pi') in Hax.
-  apply (ex_ir _ _ _ _ _ Hax)...
-- eexists.
-  apply negR_irr in pi'.
-  apply (plus_irr2 _ _ (negR R (trans R B))) in pi'.
-  apply (lmap_ilr _ _ _ _ _ _ _ _ _ pi') in Hax.
-  apply (ex_ir _ _ _ _ _ Hax)...
-- eexists.
-  rewrite <- (app_nil_l (iplus _ _ :: _)).
+- apply negR_irr in IHHll.
+  apply (plus_irr1 _ _ (negR R (trans R B))) in IHHll.
+  apply (lmap_ilr _ _ _ _ _ _ _ IHHll) in Hax.
+  apply (ex_ir _ _ _ _ Hax)...
+- apply negR_irr in IHHll.
+  apply (plus_irr2 _ _ (negR R (trans R B))) in IHHll.
+  apply (lmap_ilr _ _ _ _ _ _ _ IHHll) in Hax.
+  apply (ex_ir _ _ _ _ Hax)...
+- rewrite <- (app_nil_l (iplus _ _ :: _)).
   apply plus_ilr...
-- eexists.
-  simpl in pi' ; rewrite map_map in pi'.
-  simpl in pi' ; rewrite <- map_map in pi'.
-  apply negR_irr in pi'.
-  apply oc_irr in pi'.
+- simpl in IHHll ; rewrite map_map in IHHll.
+  simpl in IHHll ; rewrite <- map_map in IHHll.
+  apply negR_irr in IHHll.
+  apply oc_irr in IHHll.
   apply negR_ilr...
   eapply ex_ir...
   list_simpl...
   rewrite ? map_map...
-- eexists.
-  rewrite <- (app_nil_l (ioc _ :: _)).
+- rewrite <- (app_nil_l (ioc _ :: _)).
   apply de_ilr...
-  eapply ex_ir ; [ | apply Permutation_middle ].
+  eapply ex_ir ; [ | apply Permutation_Type_middle ].
   apply negR_ilr...
   apply negR_irr.
   eapply ex_ir...
-- eexists.
-  rewrite <- (app_nil_l (ioc _ :: _)).
+- rewrite <- (app_nil_l (ioc _ :: _)).
   apply wk_ilr...
-- eexists.
-  rewrite <- (app_nil_l (ioc _ :: _)).
+- rewrite <- (app_nil_l (ioc _ :: _)).
   change nil with (map ioc nil).
   rewrite <- (app_nil_l (map _ _ ++ _)).
   apply co_ilr.
   eapply ex_ir...
-- apply negR_irr in pi1'.
-  apply negR_irr in pi2'.
-  destruct (trans_dual R A) as [s0 pi0].
+- apply negR_irr in IHHll1.
+  apply negR_irr in IHHll2.
+  assert (pi0 := trans_dual R A).
   rewrite <- (app_nil_l _) in pi0.
-  eapply (cut_ir _ _ _ _ _ _ _ _ pi2') in pi0.
+  eapply (cut_ir _ _ _ _ _ _ IHHll2) in pi0.
   list_simpl in pi0.
-  eapply (cut_ir _ _ _ _ _ _ _ _ pi1') in pi0.
-  eexists.
+  eapply (cut_ir _ _ _ _ _ _ IHHll1) in pi0.
   eapply ex_ir...
-- destruct H ; subst.
+- destruct a ; subst.
   + apply ie_dual_diag...
   + simpl.
-    destruct (ie_ie_diag R Hie) as [s HR].
-    eexists.
-    eapply ex_ir ; [ | apply perm_swap ].
+    eapply ex_ir ; [ | apply Permutation_Type_swap ].
     rewrite <- 2 (app_nil_l (negR _ _ :: _)).
     apply lmap_ilr...
     * apply one_irr.
-    * eapply ex_ir...
+    * eapply ex_ir.
+      -- apply ie_ie_diag...
+      -- PEperm_Type_solve.
 Unshelve. all : reflexivity.
 Qed.
 
@@ -1023,48 +822,39 @@ Definition n2n_a := yalla_ax.n2n_a.
  - the sequent is provable in [ll].
 *)
 
-Theorem ill_trans_to_llR_bot : forall l s,
-  (forall R, ill_ll (map (trans R) l) R s) -> exists s', llR bot l s'.
-Proof with myeeasy ; try PCperm_solve.
-intros l s Hill.
+Theorem ill_trans_to_llR_bot : forall l,
+  (forall R, ill_ll (map (trans R) l) R) -> llR bot l.
+Proof with myeeasy ; try PCperm_Type_solve.
+intros l Hill.
 remember (fresh_of_list a2n n2a l) as z.
 specialize Hill with (ivar (a2i z)).
 apply ill_trans_to_llR in Hill...
-destruct Hill as [s' Hill].
 apply (subs_llR _ bot z) in Hill ; subst.
-clear s' ; destruct Hill as [s' Hill].
-eexists.
 simpl in Hill.
 rewrite repl_at_eq in Hill...
 rewrite (subs_fresh_list _ _ n2n_a) in Hill...
 Qed.
 
-Theorem llR_bot_to_ll : forall l s, llR bot l s -> exists s', ll_ll l s'.
+Theorem llR_bot_to_ll : forall l, llR bot l -> ll_ll l.
 Proof with myeeasy.
-intros l s HR.
+intros l HR.
 induction HR ;
-  try (inversion f ; fail) ;
-  try (destruct IHHR as [s' IHHR]) ;
-  try (destruct IHHR1 as [s1' IHHR1]) ;
-  try (destruct IHHR2 as [s2' IHHR2]) ;
-  try (eexists ; constructor ; myeeasy ; fail).
-- eexists.
-  eapply ex_r...
+  (try now (inversion f)) ;
+  try now constructor.
+- eapply ex_r...
 - eapply cut_ll_r...
-- inversion H ; subst.
-  + eexists.
-    apply one_r.
-  + eexists.
-    apply bot_r.
+- destruct a.
+  + apply one_r.
+  + apply bot_r.
     apply one_r.
 Qed.
 
-Theorem ll_ll_to_ill_trans : forall R l s,
-  ll_ll l s -> exists s', ill_ll (map (trans R) l) R s'.
+Theorem ll_ll_to_ill_trans : forall R l,
+  ll_ll l -> ill_ll (map (trans R) l) R.
 Proof.
-intros R l s Hll.
+intros R l Hll.
 eapply ll_to_ill_trans ; myeeasy.
-- intros l' Hax ; inversion Hax.
+- intros a ; destruct a.
 - intros f ; inversion f.
 - intros f ; inversion f.
 Qed.
@@ -1078,64 +868,48 @@ Qed.
  - the sequent is provable in [ll_mix02].
 *)
 
-Lemma ill_trans_to_llR_one : forall l s,
-  ill_ll (map (trans ione) l) ione s -> exists s', llR one l s'.
+Lemma ill_trans_to_llR_one : forall l,
+  ill_ll (map (trans ione) l) ione -> llR one l.
 Proof.
 apply ill_trans_to_llR.
 Qed.
 
-Theorem llR_one_to_ll_mix02 : forall l s,
-  llR one l s -> exists s', ll_mix02 l s'.
+Theorem llR_one_to_ll_mix02 : forall l, llR one l -> ll_mix02 l.
 Proof with myeeasy.
-intros l s pi.
-induction pi ;
-  try (destruct IHpi as [s' pi']) ;
-  try (destruct IHpi1 as [s1' pi1']) ;
-  try (destruct IHpi2 as [s2' pi2']) ;
-  try (eexists ; constructor ; myeeasy ; fail).
-- eexists.
-  eapply ex_r...
+intros l pi.
+induction pi ; try now constructor.
+- eapply ex_r...
 - eapply cut_mix02_r...
-- destruct H ; subst.
-  + eexists.
-    apply bot_r.
-    apply (@mix0_r _ (eq_refl (pmix0 pfrag_mix02))).
-  + eexists.
-    change (one :: one :: nil) with ((one :: nil) ++ (one :: nil)).
-    apply (@mix2_r _ (eq_refl (pmix2 pfrag_mix02))) ;
-    apply one_r.
+- destruct a ; simpl.
+  + apply bot_r.
+    apply mix0_r...
+  + change (one :: one :: nil) with ((one :: nil) ++ (one :: nil)).
+    apply mix2_r ; try apply one_r...
 Qed.
 
-Theorem ll_mix02_to_ill_trans : forall l s,
-  ll_mix02 l s -> exists s', ill_ll (map (trans ione) l) ione s'.
+Theorem ll_mix02_to_ill_trans : forall l,
+  ll_mix02 l -> ill_ll (map (trans ione) l) ione.
 Proof with myeeasy.
-intros l s Hll.
-eapply ll_to_ill_trans ; myeeasy ; myeeasy.
-- intros l' Hax ; inversion Hax.
+intros l Hll.
+eapply ll_to_ill_trans ; myeeasy.
+- intros a ; destruct a.
 - intros f.
-  eexists.
   apply one_irr.
-- intros f l1 l2 s1 s2 pi1 pi2.
+- intros f l1 l2 pi1 pi2.
   rewrite <- (app_nil_l (map _ l2 ++ map _ l1)).
   rewrite <- (app_nil_r (map _ l2 ++ map _ l1)).
-  assert (forall l C, ~ ipgax ipfrag_ill l C)
-     as I_axfree by (intros ? ? Hgax ; inversion Hgax).
-  eapply (@cut_ir_nzeropos_axfree_by_ll _ i2ac_inj _ I_axfree (itens ione ione)).
+eapply cut_ir_nzeropos_axfree_by_ll.
+  + apply i2ac_inj.
+  + intros ; destruct a.
   + list_simpl ; constructor.
     * constructor.
-    * apply Forall_app.
-      -- apply Forall_forall.
-         intros x Hin.
-         apply in_map_iff in Hin.
-         destruct Hin as (y & Heq & _) ; subst.
+    * apply Forall_Type_app.
+      -- clear ; induction l2 ; constructor...
          apply trans_nz.
          ++ intros Hz.
             inversion Hz.
          ++ constructor.
-      -- apply Forall_forall.
-         intros x Hin.
-         apply in_map_iff in Hin.
-         destruct Hin as (y & Heq & _) ; subst.
+      -- clear ; induction l1 ; constructor...
          apply trans_nz.
          ++ intros Hz.
             inversion Hz.
@@ -1155,27 +929,25 @@ Qed.
  - the sequent is provable in [llR zero].
 *)
 
-Lemma ill_trans_to_llR_zero : forall l s,
-  ill_ll (map (trans izero) l) izero s -> exists s', llR zero l s'.
+Lemma ill_trans_to_llR_zero : forall l,
+  ill_ll (map (trans izero) l) izero -> llR zero l.
 Proof.
 apply ill_trans_to_llR.
 Qed.
 
-Lemma llR_zero_to_ill_trans : forall l s,
-  llR zero l s -> exists s', ill_ll (map (trans izero) l) izero s'.
+Lemma llR_zero_to_ill_trans : forall l,
+  llR zero l -> ill_ll (map (trans izero) l) izero.
 Proof with myeeasy.
-intros l s pi.
+intros l pi.
 eapply llR_ie_to_ill_trans...
 constructor.
 Qed.
 
 (** Moreover in these systems, the general weakening rule is admissible. *)
-Lemma aff_to_ill_trans : forall l s,
-  ill_ll (map (trans izero) l) izero s -> forall A, exists s',
-  ill_ll (map (trans izero) (A :: l)) izero s'.
+Lemma aff_to_ill_trans : forall l A,
+  ill_ll (map (trans izero) l) izero -> ill_ll (map (trans izero) (A :: l)) izero.
 Proof with myeeasy.
-intros l s Hll A.
-eexists.
+intros l A Hll.
 simpl.
 cons2app.
 rewrite <- (app_nil_r (map _ _)).
@@ -1193,33 +965,24 @@ Qed.
 *)
 
 Theorem ill_trans_to_llR_wn_one : forall l,
-  (forall R s, ill_ll nil R s -> exists s', ill_ll (map (trans R) l) R s') ->
-    exists s'', llR (wn one) l s''.
-Proof with myeeasy ; try PCperm_solve.
+  (forall R, ill_ll nil R -> ill_ll (map (trans R) l) R) -> llR (wn one) l.
+Proof with myeeasy ; try PCperm_Type_solve.
 intros l Hill.
 remember (fresh_of_list a2n n2a l) as z.
-assert (exists s, ill_ll nil (ilpam (ioc (ivar (a2i z))) (ivar (a2i z))) s)
-  as [s Hz].
-{ eexists.
-  apply lpam_irr.
+assert (ill_ll nil (ilpam (ioc (ivar (a2i z))) (ivar (a2i z))))
+  as Hz.
+{ apply lpam_irr.
   apply de_ilr.
   apply ax_ir. }
-specialize Hill with (ilpam (ioc (ivar (a2i z))) (ivar (a2i z))) s.
+specialize Hill with (ilpam (ioc (ivar (a2i z))) (ivar (a2i z))).
 assert (Hz2 := Hz).
 apply Hill in Hz2 ; clear Hill.
-destruct Hz2 as [s' Hill].
-apply ill_trans_to_llR in Hill...
-clear s' ; destruct Hill as [s' Hill].
-apply (subs_llR _ bot z) in Hill ; subst.
-simpl in Hill.
-rewrite repl_at_eq in Hill ; try rewrite a2a_i...
-clear s' ; destruct Hill as [s' Hill].
-assert (Hax := @ax_exp (pfrag_llR (wn one)) (wn one)).
-destruct Hax as [sax Hax].
-eapply (llR1_R2 _ (wn one)) in Hill.
-- clear s' ; destruct Hill as [s' Hill].
-  eexists.
-  rewrite (subs_fresh_list _ _ n2n_a) in Hill...
+apply ill_trans_to_llR in Hz2...
+apply (subs_llR _ bot z) in Hz2 ; subst.
+simpl in Hz2.
+rewrite repl_at_eq in Hz2 ; try rewrite a2a_i...
+eapply (llR1_R2 _ (wn one)) in Hz2.
+- rewrite (subs_fresh_list _ _ n2n_a) in Hz2...
 - simpl.
   rewrite <- (app_nil_l (wn _ :: _)).
   apply tens_r.
@@ -1233,39 +996,32 @@ eapply (llR1_R2 _ (wn one)) in Hill.
   apply (ex_r _ (parr bot (wn one) :: oc bot :: nil))...
   apply parr_r.
   apply bot_r.
-  change (wn one) with (dual (oc bot))...
+  change (wn one) with (dual (oc bot)).
+  apply ax_exp.
 Qed.
 
-Theorem llR_wn_one_to_ll_mix0 : forall l s,
-  llR (wn one) l s -> exists s', ll_mix0 l s'.
+Theorem llR_wn_one_to_ll_mix0 : forall l, llR (wn one) l -> ll_mix0 l.
 Proof with myeeasy.
-intros l s pi.
-induction pi ;
-  try (destruct IHpi as [s' pi']) ;
-  try (destruct IHpi1 as [s1' pi1']) ;
-  try (destruct IHpi2 as [s2' pi2']) ;
-  try (eexists ; constructor ; myeeasy ; fail).
-- eexists.
-  eapply ex_r...
+intros l pi.
+induction pi ; try now constructor.
+- eapply ex_r...
 - eapply cut_mix0_r...
-- destruct H ; subst.
-  + eexists.
-    change nil with (map wn nil).
+- destruct a ; simpl.
+  + change nil with (map wn nil).
     apply oc_r.
     apply bot_r.
-    apply (@mix0_r _ (eq_refl (pmix0 pfrag_mix0))).
-  + eexists.
-    apply wk_r.
+    apply mix0_r...
+  + apply wk_r.
     apply one_r.
 Qed.
 
-Theorem ll_mix0_to_ill_trans : forall R l s0 s,
-  ill_ll nil R s0 -> ll_mix0 l s -> exists s', ill_ll (map (trans R) l) R s'.
+Theorem ll_mix0_to_ill_trans : forall R l,
+  ill_ll nil R -> ll_mix0 l -> ill_ll (map (trans R) l) R.
 Proof with myeeasy.
-intros R l s0 s HR Hll.
-eapply ll_to_ill_trans ; myeeasy ; myeeasy.
-- intros l' Hax ; inversion Hax.
-- intros f ; eexists...
+intros R l HR Hll.
+eapply ll_to_ill_trans ; myeeasy.
+- intros a ; destruct a.
+- intros f...
 - intros f ; inversion f.
 Qed.
 
@@ -1279,142 +1035,113 @@ Qed.
 *)
 
 Theorem ill_trans_to_llR_oc_bot : forall l,
-  (forall R, exists s, ill_ll (map (trans (ioc R)) l) (ioc R) s) ->
-  exists s', llR (oc bot) l s'.
-Proof with myeeasy ; try PCperm_solve.
+  (forall R, ill_ll (map (trans (ioc R)) l) (ioc R)) ->
+  llR (oc bot) l.
+Proof with myeeasy ; try PCperm_Type_solve.
 intros l Hill.
 remember (fresh_of_list a2n n2a l) as z.
 specialize Hill with (ivar (a2i z)).
-destruct Hill as [s Hill].
 apply ill_trans_to_llR in Hill...
-clear s ; destruct Hill as [s Hill].
 apply (subs_llR _ bot z) in Hill ; subst.
-clear s ; destruct Hill as [s Hill].
-eexists.
 simpl in Hill.
 rewrite repl_at_eq in Hill...
 rewrite (subs_fresh_list _ _ n2n_a) in Hill...
 Qed.
 
-Theorem llR_oc_bot_to_ll_bbb : forall l s,
-  llR (oc bot) l s -> exists s', ll_bbb l s'.
+Theorem llR_oc_bot_to_ll_bbb : forall l, llR (oc bot) l -> ll_bbb l.
 Proof.
 apply bb_to_bbb.
 Qed.
 
-Lemma ll_mix02_to_ill_trans_gen : forall R l s,
- ll_mix02 l s -> exists s',
-   ill_ll (ioc R :: map (trans (ioc R)) l) (ioc R) s'.
+Lemma ll_mix02_to_ill_trans_gen : forall R l,
+ ll_mix02 l -> ill_ll (ioc R :: map (trans (ioc R)) l) (ioc R).
 Proof with myeeasy.
-intros R l s Hll.
-assert (Hax := @ax_exp_ill ipfrag_ill (ioc R)).
-destruct Hax as [sax Hax].
+intros R l Hll.
 change (ioc R :: map (trans _) l)
   with (map ioc (R :: nil) ++ map (trans (ioc R)) l).
 eapply ll_to_ill_trans_gen ; intros ; simpl...
-- intro Hgax ; inversion Hgax.
-- eexists...
+- destruct a.
+- apply ax_exp_ill.
 - rewrite <- (app_nil_l (ioc R :: _)).
   rewrite <- (app_nil_r (map _ l1)).
   rewrite app_comm_cons.
   rewrite (app_assoc _ (map _ l1)).
-  assert (forall l C, ~ ipgax ipfrag_ill l C)
-     as I_axfree by (intros ? ? Hgax ; inversion Hgax).
-  eexists.
-  assert (ipcut ipfrag_ill = true) as Hcut' by (simpl ; assumption).
-  apply (@cut_ir _ Hcut' (itens (ioc R) (ioc R))).
+eapply (cut_ir _ (itens (ioc R) (ioc R))).
   + rewrite <- 2 (app_nil_l (ioc R :: _)).
     rewrite <- ? app_assoc.
     change nil with (map ioc nil) at 2.
     apply co_ilr.
     eapply ex_ir.
-    * apply tens_irr ; [ apply H0 | apply H1 ].
-    * PEperm_solve.
+    * apply tens_irr ; [ apply X | apply X0 ].
+    * PEperm_Type_solve.
   + apply tens_ilr.
-    apply wk_ilr...
+    apply wk_ilr.
+    apply ax_exp_ill.
+Unshelve. reflexivity.
 Qed.
 
-Theorem ll_bbb_to_ill_trans : forall R l s,
-  ll_bbb l s -> exists s', ill_ll (map (trans (ioc R)) l) (ioc R) s'.
-Proof with myeeasy ; try PEperm_solve.
-intros R l s Hll.
+Theorem ll_bbb_to_ill_trans : forall R l,
+  ll_bbb l -> ill_ll (map (trans (ioc R)) l) (ioc R).
+Proof with myeeasy ; try PEperm_Type_solve ; try now (apply ax_exp_ill).
+intros R l Hll.
+(*
 destruct (@ax_exp_ill ipfrag_ill (ioc R)) as [sax Hax].
 rewrite <- (app_nil_l (ioc R :: _)) in Hax.
-induction Hll ; 
-  try (inversion f ; fail) ;
-  try (inversion H ; fail) ;
-  try (destruct IHHll as [s' pi']) ;
-  try (destruct IHHll1 as [s1' pi1']) ;
-  try (destruct IHHll2 as [s2' pi2']) ;
-  simpl.
-- eexists.
-  eapply ex_ir.
-  + eapply lmap_ilr ; [ | apply Hax ].
-    eapply (ax_ir _ (a2i X)).
-  + PEperm_solve.
-- eexists.
-  eapply ex_ir...
-  apply Permutation_map...
-- apply (ll_mix02_to_ill_trans_gen R) in H.
-  destruct H as [s'' H].
-  rewrite <- (app_nil_l (ioc _ :: _)) in H.
+*)
+induction Hll ; (try now (inversion f)) ; simpl.
+- eapply ex_ir.
+  + eapply lmap_ilr ; [ | ].
+    * eapply (ax_ir _ (a2i X)).
+    * rewrite app_nil_l...
+  + PEperm_Type_solve.
+- eapply ex_ir...
+  apply Permutation_Type_map...
+- apply (ll_mix02_to_ill_trans_gen R) in l.
+  rewrite <- (app_nil_l (ioc _ :: _)) in l.
   rewrite map_app.
-  eexists.
   assert (ipcut ipfrag_ill = true) as Hcut by reflexivity.
   rewrite <- (app_nil_r (map _ l1)).
   apply (@cut_ir _ Hcut (ioc R))...
-  eapply ex_ir ; [ | apply Permutation_app_comm ]...
-- eexists.
-  apply negR_ilr...
+  eapply ex_ir ; [ | apply Permutation_Type_app_comm ]...
+- apply negR_ilr...
   apply one_irr.
-- eexists.
-  rewrite <- (app_nil_l (ione :: _)).
+- rewrite <- (app_nil_l (ione :: _)).
   apply one_ilr...
-- eexists.
-  apply negR_ilr...
+- apply negR_ilr...
   list_simpl.
-  eapply ex_ir ; [ | apply Permutation_app_comm ].
+  eapply ex_ir ; [ | apply Permutation_Type_app_comm ].
   apply tens_irr ; apply negR_irr ; eapply ex_ir.
-  + apply pi1'.
-  + PEperm_solve.
-  + apply pi2'.
-  + PEperm_solve.
-- eexists.
-  rewrite <- (app_nil_l (itens _ _ :: _)).
+  + apply IHHll1.
+  + PEperm_Type_solve.
+  + apply IHHll2.
+  + PEperm_Type_solve.
+- rewrite <- (app_nil_l (itens _ _ :: _)).
   apply tens_ilr...
-- eexists.
-  rewrite <- (app_nil_l (izero :: _)).
+- rewrite <- (app_nil_l (izero :: _)).
   apply zero_ilr.
-- eexists.
-  apply negR_ilr...
+- apply negR_ilr...
   apply plus_irr1 ; apply negR_irr ; eapply ex_ir...
-- eexists.
-  apply negR_ilr...
+- apply negR_ilr...
   apply plus_irr2 ; apply negR_irr ; eapply ex_ir...
-- eexists.
-  rewrite <- (app_nil_r (map _ _)).
+- rewrite <- (app_nil_r (map _ _)).
   rewrite <- (app_nil_l (iplus _ _ :: _)).
-  apply plus_ilr ; eapply ex_ir ; [ apply pi1' | | apply pi2' | ]...
-- eexists.
-  apply negR_ilr...
+  apply plus_ilr ; eapply ex_ir ; [ apply IHHll1 | | apply IHHll2 | ]...
+- apply negR_ilr...
   rewrite map_map ; simpl.
   rewrite <- map_map.
-  simpl in pi' ; rewrite map_map in pi'.
-  simpl in pi' ; rewrite <- map_map in pi'.
+  simpl in IHHll ; rewrite map_map in IHHll.
+  simpl in IHHll ; rewrite <- map_map in IHHll.
   apply oc_irr.
   apply negR_irr.
   eapply ex_ir...
-- eexists.
-  rewrite <- (app_nil_l (ioc _ :: _)).
+- rewrite <- (app_nil_l (ioc _ :: _)).
   apply de_ilr...
   list_simpl.
   apply negR_ilr...
   apply negR_irr...
-- eexists.
-  rewrite <- (app_nil_l (ioc _ :: _)).
+- rewrite <- (app_nil_l (ioc _ :: _)).
   apply wk_ilr...
-- eexists.
-  rewrite <- 2 (app_nil_l (ioc _ :: _)).
+- rewrite <- 2 (app_nil_l (ioc _ :: _)).
   change nil with (map ioc nil).
   apply co_ilr.
   eapply ex_ir...
@@ -1422,12 +1149,12 @@ Qed.
 
 (** The following result is the converse of [bb_to_bbb] proved in the [bbb] library *)
 
-Theorem bbb_to_bb : forall l s, ll_bbb l s -> exists s', llR (oc bot) l s'.
+Theorem bbb_to_bb : forall l, ll_bbb l -> llR (oc bot) l.
 Proof.
-intros l s pi.
+intros l pi.
 apply ill_trans_to_llR_oc_bot.
 intros R.
-eapply ll_bbb_to_ill_trans ; eassumption.
+apply ll_bbb_to_ill_trans ; eassumption.
 Qed.
 
 
